concurrency/framework/ThreadUtils.s.dfy
@@ -1,0 +1,3 @@
+module ThreadUtils {
+  method {:extern} thread_yield()
+}
